execution/tests/EIP20Tests/EIP20TokenBuggyTests.v
@@ -1,0 +1,150 @@
+Global Set Warnings "-extraction-logical-axiom".
+
+Require Import ZArith Strings.String.
+From QuickChick Require Import QuickChick. Import QcNotation.
+
+From ConCert Require Import Blockchain.
+From ConCert Require Import Serializable.
+From ConCert Require Import BoundedN.
+From ConCert Require Import Containers.
+From ConCert Require Import EIP20Token EIP20Token_Buggy.
+From ConCert Require Import ResultMonad.
+Require Import Extras.
+
+From ConCert.Execution.QCTests Require Import
+  TestUtils ChainPrinters SerializablePrinters EIP20TokenPrinters EIP20TokenGens TraceGens.
+
+From Coq Require Import List. 
+Import ListNotations.
+Import BoundedN.Stdpp.
+Import LocalBlockchain.
+
+(* -------------------------- Tests of the Buggy EIP20 Token Implementation -------------------------- *)
+
+Existing Instance showTokenState.
+
+Definition token_setup := EIP20Token.build_setup creator (100%N).
+Definition deploy_eip20token := create_deployment 0 EIP20Token_Buggy.contract token_setup.
+
+Definition token_caddr := BoundedN.of_Z_const AddrSize 128%Z.
+
+(* In the initial chain we transfer some assets to a few accounts, just to make the addresses
+   present in the chain state. The amount transferred is irrelevant. *)
+Definition token_cb :=
+  ResultMonad.unpack_result (TraceGens.add_block (lcb_initial AddrSize)
+  [
+    build_act creator (act_transfer person_1 0);
+    build_act creator (act_transfer person_2 0);
+    build_act creator (act_transfer person_3 0);
+    build_act creator deploy_eip20token
+  ]).
+
+Module TestInfo <: EIP20GensInfo.
+  Definition contract_addr := token_caddr.
+  Definition gAccount (c : Chain) := elems [person_1; person_2; person_3; person_4; person_5].
+End TestInfo.
+Module MG := EIP20Gens TestInfo. Import MG.
+
+Definition gTokenChain max_acts_per_block token_cb max_length := 
+  let act_depth := 1 in 
+  gChain token_cb
+    (fun env act_depth => gEIP20TokenAction env) max_length act_depth max_acts_per_block.
+(* Sample (gTokenChain 2 token_cb 7).  *)
+
+Definition forAllTokenChainTraces n :=
+  let max_acts_per_block := 2 in
+  forAllChainState n token_cb (gTokenChain max_acts_per_block).
+
+Instance genBuggyTokenChainSized : GenSized ChainBuilder := {
+  arbitrarySized n := gTokenChain 2 token_cb n
+}.
+
+Definition pre_post_assertion_token P c Q :=
+  let max_acts_per_block := 1 in
+  let trace_length := 5 in
+  pre_post_assertion trace_length token_cb (gTokenChain max_acts_per_block) EIP20Token_Buggy.contract c P Q.
+
+Notation "{{ P }} c {{ Q }}" := (pre_post_assertion_token P c Q) ( at level 50).
+
+Definition msg_is_transfer_from (cstate : EIP20Token.State) (msg : EIP20Token.Msg) :=
+  match msg with
+  | transfer_from _ _ _ => true
+  | _ => false
+  end.
+
+Definition checker_get_state {prop} `{Checkable prop} (pf : State -> prop) (cs : ChainState) : Checker := 
+  match get_contract_state EIP20Token.State cs token_caddr with
+  | Some state => checker (pf state)
+  | None => checker true (* trivially true case *) 
+  end.
+
+Definition get_state (pf : State -> bool) (cs : ChainState) : bool := 
+  match get_contract_state EIP20Token.State cs token_caddr with
+  | Some state => pf state
+  | None => true (* trivially true case *) 
+  end.
+
+
+Open Scope N_scope.
+Open Scope string_scope.
+(* One key property: the sum of the balances is always equal to the initial supply *)
+Definition sum_balances_eq_init_supply_checker (state : EIP20Token.State) :=
+  let balances_list := (map snd o FMap.elements) state.(balances) in
+  let balances_sum : N := fold_left N.add balances_list 0%N in
+  whenFail (
+    "balances_sum: " ++ show balances_sum ++ nl ++
+    "total_supply: " ++ show state.(total_supply) ++ nl ++
+    "balances: " ++ show state.(balances)
+    )
+  (balances_sum =? state.(total_supply))%N.
+Close Scope string_scope.
+
+Definition sum_balances_eq_init_supply (state : EIP20Token.State) : bool :=
+  let balances_list := (map snd o FMap.elements) state.(balances) in
+  let balances_sum : N := fold_left N.add balances_list 0%N in
+  (balances_sum =? state.(total_supply))%N.
+
+Conjecture token_supply_preserved : forall sig_to : {to | reachable to}, 
+  let to := proj1_sig sig_to in
+  get_state sum_balances_eq_init_supply to = true.
+
+(* QuickChick token_supply_preserved. *)
+(* *** Failed after 11 tests and 1000 shrinks. (0 discards)
+       on transfer_from 10%256 10%256 4 *)
+(* or alternatively: *)
+(* QuickChick (forAllTokenChainTraces 4 (checker_get_state sum_balances_eq_init_supply)). *)
+
+Definition transfer_balance_update_correct old_state new_state from to tokens :=
+  let get_balance addr state := with_default 0 (FMap.find addr state.(balances)) in
+  let from_balance_before := get_balance from old_state in
+  let to_balance_before := get_balance to old_state in
+  let from_balance_after := get_balance from new_state in
+  let to_balance_after := get_balance to new_state in
+  (* if the transfer is a self-transfer, balances should remain unchained *)
+  if address_eqb from to
+  then
+    (from_balance_before =? from_balance_after) &&
+    (to_balance_before =? to_balance_after)
+  else
+    (from_balance_before =? from_balance_after + tokens) &&
+    (to_balance_before + tokens =? to_balance_after).
+
+Definition post_transfer_from_correct (cctx : ContractCallContext) 
+                                      (old_state : State) 
+                                      (msg : Msg) 
+                                      (result_opt : option (State * list ActionBody)) 
+                                      : Checker :=
+  match (result_opt, msg) with
+  | (Some (new_state, _), transfer_from from to tokens) =>
+    whenFail (show msg ++ nl ++ show old_state ++ nl ++ show result_opt)
+    (checker (transfer_balance_update_correct old_state new_state from to tokens))
+  (* if 'receive' failed, or msg is not a transfer_from
+     then just discard this test *)
+  | _ => checker false
+  end.
+
+(* QuickChick (
+  {{msg_is_transfer_from}}
+  token_caddr
+  {{post_transfer_from_correct}}
+). *)
